lib/steel/pulse/Pulse.Main.fst
@@ -13,45 +13,65 @@ open Pulse.Soundness
 module Cfg = Pulse.Config
 module RU = Pulse.RuntimeUtils
 module P = Pulse.Syntax.Printer
-
+module Rec = Pulse.Recursion
 
 let debug_main g (s: unit -> T.Tac string) : T.Tac unit =
   if RU.debug_at_level (fstar_env g) "pulse.main"
   then T.print (s ())
   else ()
-  
-let main' (t:st_term) (pre:term) (g:RT.fstar_top_env)
-  : T.Tac (r:(option R.term & option (string & R.term) & R.typ){RT.well_typed g r})
+
+let main' (nm:string) (d:decl) (pre:term) (g:RT.fstar_top_env)
+  : T.Tac (RT.dsl_tac_result_t g)
   = match Pulse.Soundness.Common.check_top_level_environment g with
     | None -> T.fail "pulse main: top-level environment does not include stt at the expected types"
     | Some g ->
-      if RU.debug_at_level (fstar_env g) "Pulse"
-      then (
-        T.print (Printf.sprintf "About to check pulse term:\n%s\n" (P.st_term_to_string t))
-      );
+      if RU.debug_at_level (fstar_env g) "Pulse" then 
+        T.print (Printf.sprintf "About to check pulse decl:\n%s\n" (P.decl_to_string d));
       let (| pre, ty, pre_typing |) = Pulse.Checker.Pure.check_tot_term g pre in
-      if eq_tm ty tm_vprop
-      then let pre_typing : tot_typing g pre tm_vprop = pre_typing in
-           match t.term with
-           | Tm_Abs _ ->
-             let rng = t.range in
-             let (| t, c, t_typing |) = Pulse.Checker.Abs.check_abs g t Pulse.Checker.check in
-             Pulse.Checker.Prover.debug_prover g
-               (fun _ -> Printf.sprintf "\ncheck call returned in main with:\n%s\n"
-                         (P.st_term_to_string t));
-             debug_main g
-               (fun _ -> Printf.sprintf "\nchecker call returned in main with:\n%s\nderivation=%s\n"
-                         (P.st_term_to_string t)
-                         (Pulse.Typing.Printer.print_st_typing t_typing));
-             let refl_t = elab_comp c in
-             let refl_e = Pulse.RuntimeUtils.embed_st_term_for_extraction #st_term t (Some rng) in
-             let blob = "pulse", refl_e in
-             soundness_lemma g t c t_typing;
-             if T.ext_getv "pulse:elab_derivation" <> ""
-             then Some (elab_st_typing t_typing), Some blob, refl_t
-             else None, Some blob, refl_t
-           | _ -> fail g (Some t.range) "main: top-level term not a Tm_Abs"
-      else fail g (Some t.range) "pulse main: cannot typecheck pre at type vprop"
+      if not (eq_tm ty tm_vprop) then
+        fail g (Some pre.range) "pulse main: cannot typecheck pre at type vprop";//fix range
+      let pre_typing : tot_typing g pre tm_vprop = pre_typing in
+      match d with
+      | FnDecl { id; isrec; body } -> begin
+        match body.term with
+        | Tm_Abs _ ->
+          let nm_orig = nm in
+          let nm =
+            if isrec
+            then "__recaux_" ^ nm
+            else nm
+          in
+          let rng = body.range in
+          let (| body, c, t_typing |) = Pulse.Checker.Abs.check_abs g body Pulse.Checker.check in
+          Pulse.Checker.Prover.debug_prover g
+            (fun _ -> Printf.sprintf "\ncheck call returned in main with:\n%s\n"
+                      (P.st_term_to_string body));
+          debug_main g
+            (fun _ -> Printf.sprintf "\nchecker call returned in main with:\n%s\nderivation=%s\n"
+                      (P.st_term_to_string body)
+                      (Pulse.Typing.Printer.print_st_typing t_typing));
+          let refl_t = elab_comp c in
+          let refl_e = Pulse.RuntimeUtils.embed_st_term_for_extraction #st_term body (Some rng) in
+          let blob = "pulse", refl_e in
+          soundness_lemma g body c t_typing;
+          let main_decl =
+            if T.ext_getv "pulse:elab_derivation" <> ""
+            then RT.mk_checked_let (fstar_env g) nm (elab_st_typing t_typing) refl_t
+            else Pulse.Reflection.Util.mk_opaque_let (fstar_env g) nm (elab_st_typing t_typing) refl_t
+          in
+          (* Set the blob *)
+          let main_decl =
+            let (chk, se, _) = main_decl in
+            (chk, se, Some blob)
+          in
+          let recursive_decls =
+            if isrec
+            then Rec.tie_knot g rng body c nm nm_orig
+            else []
+          in
+          main_decl :: recursive_decls
+        | _ -> fail g (Some body.range) "main: FnDecl body not a Tm_Abs"
+        end
 
 let join_smt_goals () : Tac unit =
   let open FStar.Tactics.V2 in
@@ -81,7 +101,7 @@ let join_smt_goals () : Tac unit =
 
   ()
 
-let main t pre : RT.dsl_tac_t = fun g ->
+let main nm t pre : RT.dsl_tac_t = fun g ->
   (* We use the SMT policy by default, to collect goals in the
   proofstate and discharge them all at the end, potentially joining
   them (see below). But it can be overriden to SMTSync by `--ext
@@ -91,7 +111,7 @@ let main t pre : RT.dsl_tac_t = fun g ->
   else
     set_guard_policy SMT;
 
-  let res = main' t pre g in
+  let res = main' nm t pre g in
 
   if ext_getv "pulse:join" = "1"
      (* || ext_getv "pulse:join" <> "" *)
@@ -100,17 +120,17 @@ let main t pre : RT.dsl_tac_t = fun g ->
     join_smt_goals();
   res
 
-[@@plugin]
 let check_pulse (namespaces:list string)
                 (module_abbrevs:list (string & string))
                 (content:string)
                 (file_name:string)
                 (line col:int)
+                (nm:string)
   : RT.dsl_tac_t
   = fun env ->
       match Pulse.ASTBuilder.parse_pulse env namespaces module_abbrevs content file_name line col with
-      | Inl st_term ->
-        main st_term tm_emp env
+      | Inl decl ->
+        main nm decl tm_emp env
 
       | Inr None ->
         T.fail "Pulse parser failed"
