lib/steel/pulse/Pulse.Syntax.Base.fst
@@ -252,3 +252,7 @@ and eq_branch (b1 b2 : pattern & st_term)
     let (p2, e2) = b2 in
     eq_pattern p1 p2 && eq_st_term e1 e2
 
+let rec st_term_arity (s:st_term) =
+  match s.term with
+  | Tm_Abs {body} -> 1 + st_term_arity body
+  | _ -> 0
