lib/steel/pulse/Pulse.Recursion.fst
@@ -1,0 +1,37 @@
+module Pulse.Recursion
+
+module R = FStar.Reflection.V2
+module RT = FStar.Reflection.Typing
+open FStar.Tactics.V2
+
+open Pulse.Syntax
+open Pulse.Typing
+module P = Pulse.Syntax.Printer
+
+let tie_knot (g : env)  (rng : R.range)
+             (body : st_term) (c : comp)
+             (nm : string) (nm_orig : string)
+: Tac (list (RT.sigelt_for (fstar_env g)))
+=
+  (* This is a temporary implementation. It will just create
+  a new letbinding at the appropriate type with a `magic()` body. *)
+
+  let f_ty : host_term =
+    match c with
+    | C_Tot t ->
+      begin match t.t with
+      | Tm_FStar t -> t
+      | _ -> fail g (Some rng) "not a Tm_Fstar?"
+      end
+    | _ -> fail g (Some rng) "not a C_Tot?"
+  in
+
+  let bs, c = collect_arr_ln_bs f_ty in
+  if Nil? bs then
+    fail g (Some rng) "no binders";
+  if Nil? (List.Tot.Base.init bs) then
+    fail g (Some rng) "only one binder??";
+
+  let ty = Reflection.V2.Derived.mk_arr_ln (List.Tot.Base.init bs) c in
+
+  [RT.mk_unchecked_let (fstar_env g) nm_orig (`(magic())) ty]
