lib/steel/pulse/Pulse.Recursion.fsti
@@ -1,0 +1,13 @@
+module Pulse.Recursion
+
+module R = FStar.Reflection.V2
+module RT = FStar.Reflection.Typing
+
+open FStar.Tactics.V2
+open Pulse.Syntax
+open Pulse.Typing
+
+val tie_knot (g : env)  (rng : R.range)
+             (body : st_term) (c : comp)
+             (nm : string) (nm_orig : string)
+: Tac (list (RT.sigelt_for (fstar_env g)))
